rocq/theories/TypeSystem/CheckerUsageSoundness.v
@@ -11,7 +11,7 @@ Lemma ctx_is_ok_linear_used : forall x T Γ,
   ctx_is_ok x T Γ ->
   exists Tx st,
     ctx_lookup_state x Γ = Some (Tx, st) /\
-    (st_consumed st = true \/ path_conflicts_any_b [] (st_moved_paths st) = true).
+    st_consumed st = true.
 Proof.
   intros x T Γ Hlin Hok.
   unfold ctx_is_ok in Hok.
@@ -28,7 +28,7 @@ Lemma typed_linear_let_binding_used : forall fenv Ω n Γ Γout m x T e1 e2 T2,
     typed fenv Ω n Γ e1 T1 Γ1 /\
     typed fenv Ω n (ctx_add x T m Γ1) e2 T2 Γ2 /\
     ctx_lookup_state x Γ2 = Some (Tx, st) /\
-    (st_consumed st = true \/ path_conflicts_any_b [] (st_moved_paths st) = true).
+    st_consumed st = true.
 Proof.
   intros fenv Ω n Γ Γout m x T e1 e2 T2 Htyped Hlin.
   inversion Htyped; subst.
@@ -46,7 +46,7 @@ Lemma params_ok_linear_param_used : forall ps Γ p,
   ty_usage (param_ty p) = ULinear ->
   exists Tx st,
     ctx_lookup_state (param_name p) Γ = Some (Tx, st) /\
-    (st_consumed st = true \/ path_conflicts_any_b [] (st_moved_paths st) = true).
+    st_consumed st = true.
 Proof.
   intros ps Γ p Hin Hok Hlin.
   induction ps as [| p0 ps IH].
@@ -66,7 +66,7 @@ Lemma typed_linear_param_used : forall fenv f p,
   exists T_body Γ' Tx st,
     typed fenv (fn_outlives f) (fn_lifetimes f) (params_ctx (fn_params f)) (fn_body f) T_body Γ' /\
     ctx_lookup_state (param_name p) Γ' = Some (Tx, st) /\
-    (st_consumed st = true \/ path_conflicts_any_b [] (st_moved_paths st) = true).
+    st_consumed st = true.
 Proof.
   intros fenv f p Htyped_fn Hin Hlin.
   destruct Htyped_fn as [T_body [Γ' [Hbody [_ Hparams]]]].
@@ -116,7 +116,7 @@ Fixpoint expr_linear_lets_used (fenv : list fn_def) (e : expr) {struct e}
            typed fenv Ω n Γ e1 T1 Γ1 /\
            typed fenv Ω n (ctx_add x T m Γ1) e2 T2 Γ2 /\
            ctx_lookup_state x Γ2 = Some (Tx, st) /\
-           (st_consumed st = true \/ path_conflicts_any_b [] (st_moved_paths st) = true)) /\
+           st_consumed st = true) /\
       expr_linear_lets_used fenv e1 /\
       expr_linear_lets_used fenv e2
   | ELetInfer _ _ e1 e2 =>
@@ -169,7 +169,7 @@ Theorem infer_checked_fn_linear_params_used : forall fenv f p,
   exists T_body Γ' Tx st,
     typed fenv (fn_outlives f) (fn_lifetimes f) (params_ctx (fn_params f)) (fn_body f) T_body Γ' /\
     ctx_lookup_state (param_name p) Γ' = Some (Tx, st) /\
-    (st_consumed st = true \/ path_conflicts_any_b [] (st_moved_paths st) = true).
+    st_consumed st = true.
 Proof.
   intros fenv f p Hok Hin Hlin.
   apply typed_linear_param_used; [apply infer_fn_def_ok_sound | |]; assumption.
@@ -187,7 +187,7 @@ Theorem infer_checked_fn_linear_usage : forall fenv f,
       exists T_body Γ' Tx st,
         typed fenv (fn_outlives f) (fn_lifetimes f) (params_ctx (fn_params f)) (fn_body f) T_body Γ' /\
         ctx_lookup_state (param_name p) Γ' = Some (Tx, st) /\
-        (st_consumed st = true \/ path_conflicts_any_b [] (st_moved_paths st) = true)).
+        st_consumed st = true).
 Proof.
   intros fenv f Hok.
   split.
